Nits

theories/Basics/MonadPropR.v
@@ -19,7 +19,7 @@ From Coq Require Import Morphisms
 .
 
 Require Import Classical_Prop.
-(* See [PropT.v] in the Vellvm repo for the exact framework to follow with respect to typeclasses, as well as a proof of most monad laws for [PropTM (itree E)] *)
+(* See [PropT.v] in the Vellvm repo for the exact framework to follow with respect to typeclasses, as well as a proof of most monad laws for [PropT (itree E)] *)
 
 Definition agrees {A : Type} :=
     fun (x : A) (P : A -> Prop) => P x.
@@ -39,49 +39,48 @@ Open Scope relation_scope.
 Section Transformer.
 
   Variable (m : Type -> Type).
-  Context `{Monad m}.
-  Context {EQM : EqMR m}.
+  Context {Mm: Monad m}.
+  Context {EqMRm : EqmR m}.
   Context {ITERM : MonadIter m}.
-  Context {HEQP : @EqmR_OK m EQM}.
-  Context {HMLAWS : @MonadLaws m EQM _}.
-  Context {ML : @EqmRMonad _ _ _}.
+  Context {HEQP : EqmR_OK m}.
+  Context {ML : EqmRMonad m}.
 
   (* === Eqm Closure defined on definition of EQMR Instance. === *)
 
   (* Unlike in [MonadPropClosed.v] (in `prop` branch), under generalized eqm,
-     PropTM is not closed by construction.
-     Parameterizing each PropTM instance by a relation that it is closed under
+     PropT is not closed by construction.
+     Parameterizing each PropT instance by a relation that it is closed under
      would not give us a monad instance. Instead, we parameterize the `eqm`
      relation that the EqMR instance is defined under.
      One thing that we would need to resolve now, though, is how we state the EqMR
      closedness property.
    *)
-  Definition PropTM (A:Type) := (m A -> Prop).
+  Definition PropT (A:Type) := (m A -> Prop).
 
-  Definition sub_predicate {A B: Type} (R: A -> B -> Prop): PropTM A -> PropTM B -> Prop :=
+  Definition sub_predicate {A B: Type} (R: A -> B -> Prop): PropT A -> PropT B -> Prop :=
     fun PA PB => forall ma, PA ma -> exists mb, PB mb /\ eqmR R ma mb.
   Notation "PA '[⊆' R ']' PB" := (sub_predicate R PA PB) (at level 80).
   (* Note: the following could me more cleanly defined as (PA [⊆ †R] PB),
      but we need to assume that (eqmR †R ≈ †(eqmR R)) then
    *)
-  Definition sub_predicate_rev {A B: Type} (R: A -> B -> Prop): PropTM A -> PropTM B -> Prop :=
+  Definition sub_predicate_rev {A B: Type} (R: A -> B -> Prop): PropT A -> PropT B -> Prop :=
     fun PA PB => forall mb, PB mb -> exists ma, PA ma /\ eqmR R ma mb.
 
   (* YZ: We probably want _some_ notion of closure here additionally in the definition of [eqm].
      Has been tried and appeared to be too strong:
    *)
-  Definition relatively_closed_by_R {A B: Type} (R: A -> B -> Prop) (PA: PropTM A) (PB: PropTM B)
+  Definition relatively_closed_by_R {A B: Type} (R: A -> B -> Prop) (PA: PropT A) (PB: PropT B)
     := forall ma mb, eqmR R ma mb -> (PA ma <-> PB mb).
 
   (* Could be tried: *)
-  Definition relatively_closed_by_R_weak {A B: Type} (R: A -> B -> Prop) (PA: PropTM A) (PB: PropTM B)
+  Definition relatively_closed_by_R_weak {A B: Type} (R: A -> B -> Prop) (PA: PropT A) (PB: PropT B)
     := forall ma mb, eqmR R ma mb -> PA ma -> PB mb ->
                 (forall (ma': m A), eqmR R ma' mb -> PA ma') /\
                 (forall (mb': m B), eqmR R ma mb' -> PB mb').
 
   (* Note that we have: *)
   Lemma relatively_closed_strong_weak:
-    forall {A B: Type} (R: A -> B -> Prop) (PA: PropTM A) (PB: PropTM B),
+    forall {A B: Type} (R: A -> B -> Prop) (PA: PropT A) (PB: PropT B),
       relatively_closed_by_R R PA PB ->
       relatively_closed_by_R_weak R PA PB.
   Proof.
@@ -94,7 +93,7 @@ Section Transformer.
   (* But not the converse (there can be a computation in PA linked to another one that is not in PB as long as it is not linked to anyone in PB *)
   (* However we have: *)
   Lemma relatively_closed_weak_bij_strong:
-    forall {A B: Type} (R: A -> B -> Prop) (PA: PropTM A) (PB: PropTM B),
+    forall {A B: Type} (R: A -> B -> Prop) (PA: PropT A) (PB: PropT B),
       PA [⊆ R] PB ->
       sub_predicate_rev R PA PB ->
       (* PB [⊆ †R] PA -> *)
@@ -107,17 +106,17 @@ Section Transformer.
     edestruct INB as (x & ? & ?); eauto; eapply REL; eauto.
   Qed.
 
-  Definition eqm_PropT : forall (A B : Type) (R: A -> B -> Prop), PropTM A -> PropTM B -> Prop :=
+  Definition eqm_PropT : forall (A B : Type) (R: A -> B -> Prop), PropT A -> PropT B -> Prop :=
     fun A B R PA PB =>
       PA [⊆ R] PB /\
       PB [⊆ †R] PA.
 
-  Global Instance EqMR_PropTM : EqMR PropTM := eqm_PropT.
+  Global Instance EqmR_PropT : EqmR PropT := {| eqmR := eqm_PropT |}.
 
   Definition ret_f {A} (a:A) := (fun (x : m A) => eqm x (ret a)).
 
   (*
-    Binding a PropTM monad (PA : PropTM A) and a continuation (K : A -> PropTM)
+    Binding a PropT monad (PA : PropT A) and a continuation (K : A -> PropT)
     intuitively means that we can have an "computational decomposition" of the
     bind on the underlying monad (i.e. mb ≈ bind ma kb), where:
 
@@ -125,7 +124,7 @@ Section Transformer.
           PA describes the nondeterministic set of computation on the first part of
        the computation, ma.
     2. [(fmap kb ma) ∈ (fmap K ma)]
-          This means that the continuation PropTM captures all the nondeterministic
+          This means that the continuation PropT captures all the nondeterministic
           computations that the monadic bind captures the continuation of.
 
     As an illustrative example, if we were to have the following bind:
@@ -137,24 +136,24 @@ Section Transformer.
        {ret 1; ret 2; ret 2}.
    *)
   Definition bind_f' :=
-  fun A B (PA : PropTM A) (K : A -> PropTM B) (mb : m B) =>
+  fun A B (PA : PropT A) (K : A -> PropT B) (mb : m B) =>
     exists (ma : m A) (kb : A -> m B),
       Monad.eqm mb (bind ma kb) /\
       (PA) ma /\
       (Functor.fmap kb ma) ∈ (Functor.fmap K ma).
 
-  Global Instance Monad_PropTM : Monad (PropTM) :=
+  Global Instance Monad_PropT : Monad (PropT) :=
     {|
       ret:= @ret_f
       ; bind := bind_f'
     |}.
 
   Import RelNotations.
-  Global Instance EqMR_OK_PropTM : @EqmR_OK PropTM EqMR_PropTM.
+  Global Instance EqmR_OK_PropT : @EqmR_OK PropT EqmR_PropT.
   split.
-  - intros A R. unfold eqmR, EqMR_PropTM, eqm'. intros RR.
+  - intros A R. unfold eqmR, EqmR_PropT, eqm_PropT. intros RR.
     split; intros mx ; exists mx; split; try assumption; try reflexivity.
-  - intros A R. unfold eqmR, EqMR_PropTM, eqm'.
+  - intros A R. unfold eqmR, EqmR_PropT, eqm'.
     intros RR. split; intros.
     + destruct H0 as (HL & HR).
       apply HR in H1.  destruct H1 as (mb & MB & MB').
@@ -162,7 +161,7 @@ Section Transformer.
     + destruct H0 as (HL & HR).
       apply HL in H1.  destruct H1 as (ma & MB & MB').
       exists ma. split. assumption. symmetry. assumption.
-  - intros A R. unfold eqmR, EqMR_PropTM, eqm'.
+  - intros A R. unfold eqmR, EqmR_PropT, eqm'.
     intros RR. split; intros.
     + destruct H0 as (HL & HR).
       destruct H1 as (KL & KR).
@@ -175,7 +174,7 @@ Section Transformer.
       apply HR in MA. destruct MA as (mc & MC & MC').
       exists mc. split. assumption. eapply transitivity; eassumption.
   - intros A B.
-    unfold eqmR, EqMR_PropTM, eqm'.
+    unfold eqmR, EqmR_PropT, eqm'.
     repeat red.
     intros C R1 R2 EQR PA1 PA2.
     (* intros Htr (MA1 & MB1) (MB2 & MC1). *)
@@ -206,13 +205,13 @@ Section Transformer.
   Lemma ret_ok : forall (A1 A2 : Type) (RA : A1 -> A2 -> Prop) (a1 : A1) (a2 : A2),
       RA a1 a2 <-> (eqmR RA (ret a1) (ret a2)).
   Proof.
-    unfold eqmR, EqMR_PropTM.
+    unfold eqmR, EqmR_PropT.
   Admitted.
 
-  Instance EqmRMonad_PropTM : @EqmRMonad PropTM _ _.
+  Instance EqmRMonad_PropT : @EqmRMonad PropT _ _.
   Proof.
-    pose proof EqMR_OK_PropTM.
-    constructor; unfold eqmR, EqMR_PropTM, eqm'.
+    pose proof EqmR_OK_PropT.
+    constructor; unfold eqmR, EqmR_PropT, eqm'.
     - apply ret_ok.
     - intros A1 A2 B1 B2 RA RB ma1 ma2 kb1 kb2 HA HB.
       split; intros mb1 mb2 RB'.
@@ -227,7 +226,7 @@ Section Transformer.
       ma ∈ P' -> (P ma <-> WP P').
 
   (* Alternative definition, based on agrees. *)
-  Definition PropTM' : Type -> Type :=
+  Definition PropT' : Type -> Type :=
     fun A => {P : m A -> Prop | closed_eqmR_agrees P}.
 
   Lemma ret_f_closed_eqmR_agrees :
@@ -238,7 +237,7 @@ Section Transformer.
   Admitted.
 
   Lemma bind_f_closed_eqmR_agrees:
-    forall A B (PA : PropTM A) (K : A -> PropTM B),
+    forall A B (PA : PropT A) (K : A -> PropT B),
       closed_eqmR_agrees (bind_f A B PA K).
   Proof.
   Admitted.
@@ -249,28 +248,28 @@ Section PropT_EqmRMonad.
 
   Variable (m: Type -> Type).
   Context `{Monad m}.
-  Context {EQMR : EqMR m}.
+  Context {EQMR : EqmR m}.
   Context {ITERM : MonadIter m}.
-  Context {HEQP: @EqMR_OK m EQMR}.
+  Context {HEQP: @EqmR_OK m EQMR}.
   Context {HM: @EqmRMonad m EQMR _}.
 
-  Instance eqmR_OK_PropT : EqmR_OK (PropTM m).
+  Instance eqmR_OK_PropT : EqmR_OK (PropT m).
 End PropT_EqmRMonad.
 
 Section Laws.
 
   Variable (m: Type -> Type).
   Context `{Monad m}.
-  Context {EQM : EqMR m}.
+  Context {EQM : EqmR m}.
   Context {ITERM : MonadIter m}.
-  Context {HEQP: @EqMR_OK m EQM}.
+  Context {HEQP: @EqmR_OK m EQM}.
   Context {HMLAWS: @MonadLaws m EQM _}.
 <<<<<<< HEAD
 
 
 
 
-  Instance eqm_MonadProp_Proper {A} (P: PropTM m A) : Proper (@eqm _ _ A ==> iff) P.
+  Instance eqm_MonadProp_Proper {A} (P: PropT m A) : Proper (@eqm _ _ A ==> iff) P.
   Proof.
     cbv. intros x y Heq.
 
@@ -280,11 +279,11 @@ Section Laws.
 >>>>>>> fa1ee28772a58325ada40f7ccc78bf8157008a24
 
   Lemma bind_ret_l:
-    forall A B (f : A -> PropTM m B) (a : A),
+    forall A B (f : A -> PropT m B) (a : A),
       eqm (bind (ret a) f) (f a).
   Proof.
     cbn; unfold bind_f, ret_f; cbn; unfold liftM.
-    intros A B k a. pose proof EqmRMonad_PropTM as PM.
+    intros A B k a. pose proof EqmRMonad_PropT as PM.
     specialize (PM m H EQM ITERM _ _ _).
     split.
     - intros x y r Heq. split.
@@ -324,7 +323,7 @@ Section Laws.
   Qed.
 
   Lemma bind_ret_r:
-    forall A (ma : PropTM m A),
+    forall A (ma : PropT m A),
       eqm (bind ma (fun x => ret x)) ma.
   Proof.
     intros A PTmA.
@@ -365,18 +364,18 @@ Section Laws.
 Admitted.
 
   Lemma bind_bind:
-    forall A B C (ma : PropTM m A) (mab : A -> PropTM m B)
-           (mbc : B -> PropTM m C),
+    forall A B C (ma : PropT m A) (mab : A -> PropT m B)
+           (mbc : B -> PropT m C),
       eqm (bind (bind ma mab) mbc) (bind ma (fun x => bind (mab x) mbc)).
   Proof.
   Admitted.
 
   Lemma respect_bind :
-  forall a b : Type, Proper (eqm ==> pointwise_relation a eqm ==> @eqm (PropTM m) _ b) bind.
+  forall a b : Type, Proper (eqm ==> pointwise_relation a eqm ==> @eqm (PropT m) _ b) bind.
   Proof.
   Admitted.
 
-  Global Instance PropTM_Laws : @MonadLaws (PropTM m) _ _.
+  Global Instance PropT_Laws : @MonadLaws (PropT m) _ _.
   split. apply bind_ret_l.
   apply bind_ret_r. apply bind_bind.
   apply respect_bind.
